Remove HReduce, use Reduce

dist/Klas_HReduce.cu
@@ -5,14 +5,14 @@ __global__
 /**
   hoisted when extracting reduce_f16_plus
 */
-static void __hoisted_reduce_f16_plus_0(uint32_t nth, uint32_t lena, half *a,
+static void __hoisted_reduce_f16_plus_0(uint32_t nth, uint32_t lena, half *x_,
                                         half *out)
 {
     half *sa = (half *) KPR_SHMEM_AT(0U);
     half acc = __float2half_rn(0.0f);
     uint32_t idx = threadIdx.x;
     for (; idx < lena; idx += nth)
-        acc = __hadd(acc, a[idx]);
+        acc = __hadd(acc, x_[idx]);
     sa[threadIdx.x] = acc;
     uint32_t n = 0U;
     for (; 1U << (uint32_t) n < nth; n++) {
@@ -25,39 +25,46 @@ static void __hoisted_reduce_f16_plus_0(uint32_t nth, uint32_t lena, half *a,
                 sa[threadIdx.x] = __hadd(sa[threadIdx.x], sa[nextid]);
     }
     if (threadIdx.x == 0U)
-        *out = *sa;
+        out[blockIdx.x] = *sa;
 }
 
 half Klas_HReduce_reduce_f16_plus(uint32_t nth, uint32_t lena, half *a)
 {
     uint64_t lena64 = (uint64_t) lena;
     KPR_ASSERT(!(lena64 + (uint64_t) nth < lena64));
-    half *out = (half *) KPR_GPU_ALLOC(sizeof(half), 1U);
+    half *x_ = a;
+    half *out0 = (half *) KPR_GPU_ALLOC(sizeof(half), 1U);
+    half *out = out0;
     KPR_SHMEM_FITS(2U * nth);
     MUST(cudaFuncSetAttribute(__hoisted_reduce_f16_plus_0,
                               cudaFuncAttributeMaxDynamicSharedMemorySize,
                               2U * nth));
-    KPR_KCALL(__hoisted_reduce_f16_plus_0, 1U, nth, 2U * nth, nth, lena, a,
+    KPR_KCALL(__hoisted_reduce_f16_plus_0, 1U, nth, 2U * nth, nth, lena, x_,
               out);
     MUST(cudaDeviceSynchronize());
-    half hout = __float2half_rn(0.0f);
-    MUST(cudaMemcpy(&hout, out, sizeof(half), cudaMemcpyDeviceToHost));
-    MUST(cudaFree(out));
-    return hout;
+    half *local_out = (half *) KRML_HOST_MALLOC(sizeof(half));
+    if (local_out != NULL)
+        *local_out = __float2half_rn(0.0f);
+    MUST(cudaMemcpy
+         (local_out, out0, (uint32_t) sizeof(half), cudaMemcpyDeviceToHost));
+    half res = *local_out;
+    KRML_HOST_FREE(local_out);
+    MUST(cudaFree(out0));
+    return res;
 }
 
 __global__
 /**
   hoisted when extracting reduce_f32_plus
 */
-static void __hoisted_reduce_f32_plus_0(uint32_t nth, uint32_t lena, float *a,
+static void __hoisted_reduce_f32_plus_0(uint32_t nth, uint32_t lena, float *x_,
                                         float *out)
 {
     float *sa = (float *)KPR_SHMEM_AT(0U);
     float acc = 0.0f;
     uint32_t idx = threadIdx.x;
     for (; idx < lena; idx += nth)
-        acc += a[idx];
+        acc += x_[idx];
     sa[threadIdx.x] = acc;
     uint32_t n = 0U;
     for (; 1U << (uint32_t) n < nth; n++) {
@@ -70,39 +77,46 @@ static void __hoisted_reduce_f32_plus_0(uint32_t nth, uint32_t lena, float *a,
                 sa[threadIdx.x] += sa[nextid];
     }
     if (threadIdx.x == 0U)
-        *out = *sa;
+        out[blockIdx.x] = *sa;
 }
 
 float Klas_HReduce_reduce_f32_plus(uint32_t nth, uint32_t lena, float *a)
 {
     uint64_t lena64 = (uint64_t) lena;
     KPR_ASSERT(!(lena64 + (uint64_t) nth < lena64));
-    float *out = (float *)KPR_GPU_ALLOC(sizeof(float), 1U);
+    float *x_ = a;
+    float *out0 = (float *)KPR_GPU_ALLOC(sizeof(float), 1U);
+    float *out = out0;
     KPR_SHMEM_FITS(4U * nth);
     MUST(cudaFuncSetAttribute(__hoisted_reduce_f32_plus_0,
                               cudaFuncAttributeMaxDynamicSharedMemorySize,
                               4U * nth));
-    KPR_KCALL(__hoisted_reduce_f32_plus_0, 1U, nth, 4U * nth, nth, lena, a,
+    KPR_KCALL(__hoisted_reduce_f32_plus_0, 1U, nth, 4U * nth, nth, lena, x_,
               out);
     MUST(cudaDeviceSynchronize());
-    float hout = 0.0f;
-    MUST(cudaMemcpy(&hout, out, sizeof(float), cudaMemcpyDeviceToHost));
-    MUST(cudaFree(out));
-    return hout;
+    float *local_out = (float *)KRML_HOST_MALLOC(sizeof(float));
+    if (local_out != NULL)
+        *local_out = 0.0f;
+    MUST(cudaMemcpy
+         (local_out, out0, (uint32_t) sizeof(float), cudaMemcpyDeviceToHost));
+    float res = *local_out;
+    KRML_HOST_FREE(local_out);
+    MUST(cudaFree(out0));
+    return res;
 }
 
 __global__
 /**
   hoisted when extracting reduce_f64_plus
 */
-static void __hoisted_reduce_f64_plus_0(uint32_t nth, uint32_t lena, double *a,
+static void __hoisted_reduce_f64_plus_0(uint32_t nth, uint32_t lena, double *x_,
                                         double *out)
 {
     double *sa = (double *)KPR_SHMEM_AT(0U);
     double acc = 0.0;
     uint32_t idx = threadIdx.x;
     for (; idx < lena; idx += nth)
-        acc += a[idx];
+        acc += x_[idx];
     sa[threadIdx.x] = acc;
     uint32_t n = 0U;
     for (; 1U << (uint32_t) n < nth; n++) {
@@ -115,25 +129,32 @@ static void __hoisted_reduce_f64_plus_0(uint32_t nth, uint32_t lena, double *a,
                 sa[threadIdx.x] += sa[nextid];
     }
     if (threadIdx.x == 0U)
-        *out = *sa;
+        out[blockIdx.x] = *sa;
 }
 
 double Klas_HReduce_reduce_f64_plus(uint32_t nth, uint32_t lena, double *a)
 {
     uint64_t lena64 = (uint64_t) lena;
     KPR_ASSERT(!(lena64 + (uint64_t) nth < lena64));
-    double *out = (double *)KPR_GPU_ALLOC(sizeof(double), 1U);
+    double *x_ = a;
+    double *out0 = (double *)KPR_GPU_ALLOC(sizeof(double), 1U);
+    double *out = out0;
     KPR_SHMEM_FITS(8U * nth);
     MUST(cudaFuncSetAttribute(__hoisted_reduce_f64_plus_0,
                               cudaFuncAttributeMaxDynamicSharedMemorySize,
                               8U * nth));
-    KPR_KCALL(__hoisted_reduce_f64_plus_0, 1U, nth, 8U * nth, nth, lena, a,
+    KPR_KCALL(__hoisted_reduce_f64_plus_0, 1U, nth, 8U * nth, nth, lena, x_,
               out);
     MUST(cudaDeviceSynchronize());
-    double hout = 0.0;
-    MUST(cudaMemcpy(&hout, out, sizeof(double), cudaMemcpyDeviceToHost));
-    MUST(cudaFree(out));
-    return hout;
+    double *local_out = (double *)KRML_HOST_MALLOC(sizeof(double));
+    if (local_out != NULL)
+        *local_out = 0.0;
+    MUST(cudaMemcpy
+         (local_out, out0, (uint32_t) sizeof(double), cudaMemcpyDeviceToHost));
+    double res = *local_out;
+    KRML_HOST_FREE(local_out);
+    MUST(cudaFree(out0));
+    return res;
 }
 
 __global__
@@ -141,14 +162,14 @@ __global__
   hoisted when extracting reduce_u32_plus
 */
 static void
-__hoisted_reduce_u32_plus_0(uint32_t nth, uint32_t lena, uint32_t *a,
+__hoisted_reduce_u32_plus_0(uint32_t nth, uint32_t lena, uint32_t *x_,
                             uint32_t *out)
 {
     uint32_t *sa = (uint32_t *) KPR_SHMEM_AT(0U);
     uint32_t acc = 0U;
     uint32_t idx = threadIdx.x;
     for (; idx < lena; idx += nth)
-        acc += a[idx];
+        acc += x_[idx];
     sa[threadIdx.x] = acc;
     uint32_t n = 0U;
     for (; 1U << (uint32_t) n < nth; n++) {
@@ -161,25 +182,31 @@ __hoisted_reduce_u32_plus_0(uint32_t nth, uint32_t lena, uint32_t *a,
                 sa[threadIdx.x] += sa[nextid];
     }
     if (threadIdx.x == 0U)
-        *out = *sa;
+        out[blockIdx.x] = *sa;
 }
 
 uint32_t Klas_HReduce_reduce_u32_plus(uint32_t nth, uint32_t lena, uint32_t *a)
 {
     uint64_t lena64 = (uint64_t) lena;
     KPR_ASSERT(!(lena64 + (uint64_t) nth < lena64));
-    uint32_t *out = (uint32_t *) KPR_GPU_ALLOC(sizeof(uint32_t), 1U);
+    uint32_t *x_ = a;
+    uint32_t *out0 = (uint32_t *) KPR_GPU_ALLOC(sizeof(uint32_t), 1U);
+    uint32_t *out = out0;
     KPR_SHMEM_FITS(4U * nth);
     MUST(cudaFuncSetAttribute(__hoisted_reduce_u32_plus_0,
                               cudaFuncAttributeMaxDynamicSharedMemorySize,
                               4U * nth));
-    KPR_KCALL(__hoisted_reduce_u32_plus_0, 1U, nth, 4U * nth, nth, lena, a,
+    KPR_KCALL(__hoisted_reduce_u32_plus_0, 1U, nth, 4U * nth, nth, lena, x_,
               out);
     MUST(cudaDeviceSynchronize());
-    uint32_t hout = 0U;
-    MUST(cudaMemcpy(&hout, out, sizeof(uint32_t), cudaMemcpyDeviceToHost));
-    MUST(cudaFree(out));
-    return hout;
+    uint32_t *local_out = (uint32_t *) KRML_HOST_CALLOC(1U, sizeof(uint32_t));
+    MUST(cudaMemcpy
+         (local_out, out0, (uint32_t) sizeof(uint32_t),
+          cudaMemcpyDeviceToHost));
+    uint32_t res = *local_out;
+    KRML_HOST_FREE(local_out);
+    MUST(cudaFree(out0));
+    return res;
 }
 
 __global__
@@ -187,14 +214,14 @@ __global__
   hoisted when extracting reduce_u64_plus
 */
 static void
-__hoisted_reduce_u64_plus_0(uint32_t nth, uint32_t lena, uint64_t *a,
+__hoisted_reduce_u64_plus_0(uint32_t nth, uint32_t lena, uint64_t *x_,
                             uint64_t *out)
 {
     uint64_t *sa = (uint64_t *) KPR_SHMEM_AT(0U);
     uint64_t acc = 0ULL;
     uint32_t idx = threadIdx.x;
     for (; idx < lena; idx += nth)
-        acc += a[idx];
+        acc += x_[idx];
     sa[threadIdx.x] = acc;
     uint32_t n = 0U;
     for (; 1U << (uint32_t) n < nth; n++) {
@@ -207,23 +234,29 @@ __hoisted_reduce_u64_plus_0(uint32_t nth, uint32_t lena, uint64_t *a,
                 sa[threadIdx.x] += sa[nextid];
     }
     if (threadIdx.x == 0U)
-        *out = *sa;
+        out[blockIdx.x] = *sa;
 }
 
 uint64_t Klas_HReduce_reduce_u64_plus(uint32_t nth, uint32_t lena, uint64_t *a)
 {
     uint64_t lena64 = (uint64_t) lena;
     KPR_ASSERT(!(lena64 + (uint64_t) nth < lena64));
-    uint64_t *out = (uint64_t *) KPR_GPU_ALLOC(sizeof(uint64_t), 1U);
+    uint64_t *x_ = a;
+    uint64_t *out0 = (uint64_t *) KPR_GPU_ALLOC(sizeof(uint64_t), 1U);
+    uint64_t *out = out0;
     KPR_SHMEM_FITS(8U * nth);
     MUST(cudaFuncSetAttribute(__hoisted_reduce_u64_plus_0,
                               cudaFuncAttributeMaxDynamicSharedMemorySize,
                               8U * nth));
-    KPR_KCALL(__hoisted_reduce_u64_plus_0, 1U, nth, 8U * nth, nth, lena, a,
+    KPR_KCALL(__hoisted_reduce_u64_plus_0, 1U, nth, 8U * nth, nth, lena, x_,
               out);
     MUST(cudaDeviceSynchronize());
-    uint64_t hout = 0ULL;
-    MUST(cudaMemcpy(&hout, out, sizeof(uint64_t), cudaMemcpyDeviceToHost));
-    MUST(cudaFree(out));
-    return hout;
+    uint64_t *local_out = (uint64_t *) KRML_HOST_CALLOC(1U, sizeof(uint64_t));
+    MUST(cudaMemcpy
+         (local_out, out0, (uint32_t) sizeof(uint64_t),
+          cudaMemcpyDeviceToHost));
+    uint64_t res = *local_out;
+    KRML_HOST_FREE(local_out);
+    MUST(cudaFree(out0));
+    return res;
 }
